erasure/theories/EAstUtils.v
@@ -1,8 +1,7 @@
-From Coq Require Import Ascii String Bool OrderedType Lia List Program Arith.
-From MetaCoq.Template Require Import utils Ast AstUtils.
+From Coq Require Import Ascii String OrderedType Arith.
+From MetaCoq.Template Require Import utils.
 From MetaCoq.Erasure Require Import EAst.
 Import List.ListNotations.
-Require Import FunctionalExtensionality.
 Require Import ssreflect ssrbool.
 
 Set Asymmetric Patterns.
