pcuic/theories/PCUICClosed.v
@@ -1,12 +1,9 @@
 (* Distributed under the terms of the MIT license.   *)
-From Equations Require Import Equations.
-From Coq Require Import Bool String List Program BinPos Compare_dec Arith Lia.
-From MetaCoq.Template Require Import config utils Ast.
-From MetaCoq.PCUIC Require Import PCUICAst PCUICAstUtils PCUICInduction PCUICLiftSubst
-     PCUICUnivSubst PCUICTyping PCUICWeakeningEnv.
+From Coq Require Import Bool List Program Arith Lia.
+From MetaCoq.Template Require Import config utils.
+From MetaCoq.PCUIC Require Import PCUICAst PCUICInduction
+     PCUICLiftSubst PCUICUnivSubst PCUICTyping PCUICWeakeningEnv.
 Require Import ssreflect ssrbool.
-
-Require Import Equations.Prop.DepElim.
 
 (** * Lemmas about the [closedn] predicate *)
 
