pcuic/theories/PCUICConversion.v
@@ -1,9 +1,8 @@
 (* Distributed under the terms of the MIT license.   *)
-From Equations Require Import Equations.
-From Coq Require Import Bool String List Program BinPos Compare_dec Lia.
-From MetaCoq.Template Require Import config utils AstUtils.
-From MetaCoq.PCUIC Require Import PCUICAst PCUICAstUtils PCUICInduction
-     PCUICLiftSubst PCUICUnivSubst PCUICTyping PCUICWeakeningEnv
+From Coq Require Import Bool List Program Lia.
+From MetaCoq.Template Require Import config utils.
+From MetaCoq.PCUIC Require Import PCUICAst
+     PCUICLiftSubst PCUICTyping
      PCUICSubstitution PCUICPosition PCUICCumulativity PCUICReduction
      PCUICConfluence  PCUICParallelReductionConfluence PCUICEquality
      PCUICContextConversion PCUICWeakening.
