pcuic/theories/PCUICCumulativity.v
@@ -1,18 +1,13 @@
 (* Distributed under the terms of the MIT license.   *)
-From Equations Require Import Equations.
-From Coq Require Import Bool String List Program BinPos Compare_dec.
-From MetaCoq.Template Require Import config utils AstUtils.
-From MetaCoq.PCUIC Require Import PCUICAst PCUICAstUtils PCUICInduction
-     PCUICLiftSubst PCUICUnivSubst PCUICEquality PCUICTyping PCUICWeakeningEnv
-     PCUICWeakening PCUICClosed PCUICReduction PCUICPosition.
-Require Import ssreflect ssrbool.
-Require Import String.
-From MetaCoq Require Import LibHypsNaming.
+
+From MetaCoq.Template Require Import config utils.
+From MetaCoq.PCUIC Require Import PCUICAst
+     PCUICEquality PCUICTyping
+     PCUICReduction PCUICPosition.
 Local Open Scope string_scope.
 Set Asymmetric Patterns.
 Require Import CRelationClasses.
 Require Import Equations.Type.Relation Equations.Type.Relation_Properties.
-Require Import Equations.Prop.DepElim.
 
 Set Default Goal Selector "!".
 
