pcuic/theories/PCUICMetaTheory.v
@@ -1,9 +1,7 @@
 (* Distributed under the terms of the MIT license.   *)
 
-From Coq Require Import Bool String List Program BinPos Compare_dec.
-From MetaCoq.Template Require Import config utils.
-From MetaCoq.PCUIC Require Import PCUICAst PCUICAstUtils PCUICInduction PCUICLiftSubst PCUICUnivSubst PCUICTyping.
-Require Import String.
+
+From MetaCoq.PCUIC Require Import PCUICAst PCUICTyping.
 Local Open Scope string_scope.
 Set Asymmetric Patterns.
 
